initial automation of simple encryption

protocols/SimpleEncProtocol.v
@@ -42,7 +42,7 @@ Section IdealProtocol.
   Definition PERMS__a := $0 $+ (CH__A2B, {| read := false; write := true |}). (* writer *)
   Definition PERMS__b := $0 $+ (CH__A2B, {| read := true; write := false |}). (* reader *)
 
-  Definition mkiU (cv : channels) (p__a p__b : cmd nat): universe nat :=
+  Definition mkiU (cv : channels) (p__a p__b : cmd (Base Nat) ): universe Nat :=
     {| channel_vector := cv
      ; users := $0
          $+ (A,   {| perms    := PERMS__a ; protocol := p__a |})
@@ -57,33 +57,24 @@ Section IdealProtocol.
          ; Return n)
          (* user B *)
          ( m <- @Recv Nat CH__A2B
-         ; Return match extractContent m with
-                  | None =>    0
-                  | Some n' => n'
-                  end).
+           ; ret (extractContent m)).
 
   Definition ideal_univ_sent1 n :=
     mkiU ($0 $+ (CH__A2B, [existT _ _ (Content n)]))
          (* user A *)
-         ( _ <- Return tt
-         ; Return n)
+         ( _ <- ret tt
+         ; ret n)
          (* user B *)
          ( m <- @Recv Nat CH__A2B
-         ; Return match extractContent m with
-                  | None =>    0
-                  | Some n' => n'
-                  end).
+             ; ret (extractContent m)).
 
   Definition ideal_univ_recd1 n :=
     mkiU ($0 $+ (CH__A2B, []))
          (* user A *)
          (Return n)
          (* user B *)
-         ( m <- Return (Content n)
-         ; Return match extractContent m with
-                  | None =>    0
-                  | Some n' => n'
-                  end).
+         ( m <- @Return (Message Nat) (Content n)
+         ; ret (extractContent m)).
 
   Definition ideal_univ_done n :=
     mkiU ($0 $+ (CH__A2B, []))
@@ -114,7 +105,7 @@ Section RealProtocol.
   Definition mkrU (mycs1 mycs2 : my_ciphers) (froms1 froms2 : recv_nonces)
                   (sents1 sents2 : sent_nonces) (cur_n1 cur_n2 : nat)
                   (msgs1 msgs2 : queued_messages) (cs : ciphers)
-                  (p__a p__b : user_cmd nat) (adv : user_data unit) : universe nat unit :=
+                  (p__a p__b : user_cmd (Base Nat)) (adv : user_data Unit) : universe Nat Unit :=
     {| users := $0
          $+ (A, {| key_heap := A__keys ; protocol := p__a ; msg_heap := msgs1 ; c_heap := mycs1
                  ; from_nons := froms1 ; sent_nons := sents1 ; cur_nonce := cur_n1 |})
@@ -134,66 +125,53 @@ Section RealProtocol.
          ; Return n)
 
          (* user B *)
-         ( c  <- @Recv Nat (SignedEncrypted KID__A KID__B)
+         ( c  <- @Recv Nat (SignedEncrypted KID__A KID__B true)
          ; v  <- Decrypt c
-         ; Return match v with
-                        | message.Content p => p
-                        | _                 => 0
-                        end).
+         ; ret (extractContent v)).
   
   Definition real_univ_sent1 n cs mycs1 mycs2 cur_n1 cur_n2 cid1 non1 :=
     mkrU mycs1 mycs2 [] [] [non1] [] cur_n1 cur_n2 [] [existT _ Nat (SignedCiphertext cid1)]
          (cs $+ (cid1, SigEncCipher KID__A KID__B B non1 (message.Content n)))
          (* user A *)
-         ( _  <- Return tt
-         ; Return n)
+         ( _  <- ret tt
+         ; ret n )
 
          (* user B *)
-         ( c  <- @Recv Nat (SignedEncrypted KID__A KID__B)
+         ( c  <- @Recv Nat (SignedEncrypted KID__A KID__B true)
          ; v  <- Decrypt c
-         ; Return match v with
-                        | message.Content p => p
-                        | _                 => 0
-                        end).
+         ; ret (extractContent v)).
 
   Definition real_univ_recd1 n cs mycs1 mycs2 cur_n1 cur_n2 cid1 non1 :=
     mkrU mycs1 mycs2 [] [non1] [non1] [] cur_n1 cur_n2 [] []
          (cs $+ (cid1, SigEncCipher KID__A KID__B B non1 (message.Content n)))
          (* user A *)
-         ( _  <- Return tt
-         ; Return n)
+         ( _  <- ret tt
+         ; ret n)
 
          (* user B *)
-         ( c  <- (Return (SignedCiphertext cid1))
+         ( c  <- (@Return (Crypto Nat) (SignedCiphertext cid1))
          ; v  <- @Decrypt Nat  c
-         ; Return match v with
-                        | message.Content p => p
-                        | _                 => 0
-                        end).
+         ; ret (extractContent v)).
 
-  Inductive RSimplePing : RealWorld.simpl_universe nat -> IdealWorld.universe nat -> Prop :=
+  Inductive RSimpleEnc : RealWorld.simpl_universe Nat -> IdealWorld.universe Nat -> Prop :=
   | Start : forall U__r cs mycs1 mycs2 cur_n1 cur_n2 adv,
-      rstepSilent^* (real_univ_start cs mycs1 mycs2 cur_n1 cur_n2 adv) U__r
-      -> lameAdv tt adv
-      -> RSimplePing (peel_adv U__r) ideal_univ_start
+      ~^* (real_univ_start cs mycs1 mycs2 cur_n1 cur_n2 adv) U__r
+      -> @lameAdv Unit tt adv
+      -> RSimpleEnc (peel_adv U__r) ideal_univ_start
   | Sent1 : forall U__r cs mycs1 mycs2 cur_n1 cur_n2 n cid1 non1 adv,
-      rstepSilent^* (real_univ_sent1 n cs mycs1 mycs2 cur_n1 cur_n2 cid1 non1 adv) U__r
-      -> lameAdv tt adv
-      -> RSimplePing (peel_adv U__r) (ideal_univ_sent1 n)
+      ~^* (real_univ_sent1 n cs mycs1 mycs2 cur_n1 cur_n2 cid1 non1 adv) U__r
+      -> @lameAdv Unit tt adv
+      -> RSimpleEnc (peel_adv U__r) (ideal_univ_sent1 n)
   | Recd1 : forall U__r cs mycs1 mycs2 cur_n1 cur_n2 n cid1 non1 adv,
-      rstepSilent^* (real_univ_recd1 n cs mycs1 mycs2 cur_n1 cur_n2 cid1 non1 adv) U__r
-      -> lameAdv tt adv
-      -> RSimplePing (peel_adv U__r) (ideal_univ_recd1 n)
-  (* | Done : forall U__r cs mycs1 mycs2 froms1 froms2 sents1 sents2 cur_n1 cur_n2 n cid1 seq1 adv, *)
-  (*     rstepSilent^* (real_univ_done n cs mycs1 mycs2 froms1 froms2 sents1 sents2 cur_n1 cur_n2 cid1 seq1 adv) U__r *)
-  (*     -> lameAdv tt adv *)
-  (*     -> RSimplePing (peel_adv U__r) (ideal_univ_done n) *)
+      ~^* (real_univ_recd1 n cs mycs1 mycs2 cur_n1 cur_n2 cid1 non1 adv) U__r
+      -> @lameAdv Unit tt adv
+      -> RSimpleEnc (peel_adv U__r) (ideal_univ_recd1 n)
   .
 
 End RealProtocol.
 
-Hint Constructors RealWorld.msg_accepted_by_pattern.
-Hint Constructors RSimplePing.
+Hint Constructors RealWorld.msg_accepted_by_pattern : core.
+Hint Constructors RSimpleEnc : core.
 
 Import SimulationAutomation.
 
@@ -202,32 +180,29 @@ Hint Unfold
      real_univ_start real_univ_sent1 real_univ_recd1  mkrU
      ideal_univ_start ideal_univ_sent1 ideal_univ_recd1 ideal_univ_done mkiU : constants.
 
-Hint Extern 0 (rstepSilent ^* _ _) =>
- progress(unfold real_univ_start, real_univ_sent1, real_univ_recd1, mkrU; simpl).
-Hint Extern 1 (RSimplePing (RealWorld.buildUniverse _ _ _ _ _ _) _) => unfold RealWorld.buildUniverse; simpl.
-Hint Extern 1 (RSimplePing (RealWorld.peel_adv _) _) => unfold RealWorld.peel_adv; simpl.
+Hint Extern 0 (~^* _ _) =>
+ progress(unfold real_univ_start, real_univ_sent1, real_univ_recd1, mkrU; simpl) : core.
+Hint Extern 1 (RSimpleEnc (RealWorld.buildUniverse _ _ _ _ _ _) _) => unfold RealWorld.buildUniverse; simpl : core.
+Hint Extern 1 (RSimpleEnc (RealWorld.peel_adv _) _) => unfold RealWorld.peel_adv; simpl : core.
 
 Hint Extern 0 (IdealWorld.lstep_universe _ _ _) =>
- progress(unfold ideal_univ_start, ideal_univ_sent1, ideal_univ_recd1, ideal_univ_done, mkiU; simpl).
+ progress(unfold ideal_univ_start, ideal_univ_sent1, ideal_univ_recd1, ideal_univ_done, mkiU; simpl) : core.
 
-Hint Extern 1 (IdealWorld.lstep_universe _ _ _) => single_step_ideal_universe; eauto 2; econstructor.
+Hint Extern 1 (IdealWorld.lstep_universe _ _ _) => single_step_ideal_universe; eauto 2; econstructor : core.
 
-(* Hint Extern 1 (KEYS $? _ = _) => unfold KEYS, A__keys, B__keys, KEY1, KEY2, KID1, KID2. *)
-(* Hint Extern 1 (A__keys $? _ = _) => unfold A__keys, B__keys, KEY1, KEY2, KID1, KID2. *)
-(* Hint Extern 1 (B__keys $? _ = _) => unfold A__keys, B__keys, KEY1, KEY2, KID1, KID2. *)
-Hint Extern 1 (PERMS__a $? _ = _) => unfold PERMS__a.
-Hint Extern 1 (PERMS__b $? _ = _) => unfold PERMS__b.
+Hint Extern 1 (PERMS__a $? _ = _) => unfold PERMS__a : core.
+Hint Extern 1 (PERMS__b $? _ = _) => unfold PERMS__b : core.
 
 Section FeebleSimulates.
 
   Hint Extern 0 (istepSilent ^* _ _) =>
-    progress(unfold ideal_univ_start, ideal_univ_sent1, ideal_univ_recd1, ideal_univ_done, mkiU; simpl).
+    progress(unfold ideal_univ_start, ideal_univ_sent1, ideal_univ_recd1, ideal_univ_done, mkiU; simpl) : core.
   Hint Extern 1 (istepSilent ^* _ _) =>
     repeat (ideal_single_silent_multistep A);
-    repeat (ideal_single_silent_multistep B); solve_refl.
+    repeat (ideal_single_silent_multistep B); solve_refl : core.
 
-  Lemma rsimpleping_silent_simulates :
-    simulates_silent_step (lameAdv tt) RSimplePing.
+  Lemma rsimpleenc_silent_simulates :
+    simulates_silent_step (@lameAdv Unit tt) RSimpleEnc.
   Proof.
     unfold simulates_silent_step.
 
@@ -241,199 +216,87 @@ Section FeebleSimulates.
       ).
   Qed.
 
-  Lemma rsimpleping_loud_simulates :
-    simulates_labeled_step (lameAdv tt) RSimplePing.
+  Lemma rsimpleenc_loud_simulates :
+    simulates_labeled_step (@lameAdv Unit tt) RSimpleEnc.
   Proof.
     unfold simulates_labeled_step.
-
-    intros * R UOK AOK LAME * STEP;
-      clear UOK AOK;
-      invert R;
-      destruct U__r0; destruct U__r; simpl in *; subst.
-
-    - churn.
-      
-      do 3 eexists;
-        repeat (apply conj);
-        swap 3 4; swap 2 3; swap 1 2;
-       simpl; clean_map_lookups;
-         eauto; eauto 12.
-
-      simpl_real_users_context.
-      simpl_ideal_users_context.
-      eapply Out; simpl; auto.
-      eapply CryptoSigEncCase; simpl; eauto. reflexivity.
-      econstructor.  (* pull in master*)
-      intros. unfold PERMS__b in H1. unfold PERMS__a in H1. churn.
-      split_ands. in H7; intros; eauto.
-
-      apply lookup_some_implies_in in H1; simpl in H1; split_ors; try contradiction;
-        invert H1; clean_map_lookups; eauto.
-      simpl. unfold PERMS__a; clean_map_lookups; eauto.
-
-      
-      shelve. split.
-
-      apply lookup_some_implies_in in H1; simpl in H1; split_ors; try contradiction;
-        invert H1; clean_map_lookups; simpl; eauto.
-      
-      apply lookup_some_implies_in in H1; simpl in H1; split_ors; try contradiction;
-        invert H1; clean_map_lookups; simpl; eauto.
-
-      simpl in *. shelve. 
-
-    - churn.
-      + do 3 eexists;
+    time (
+        intros * R UOK AOK LAME * STEP;
+        clear UOK AOK;
+        invert R;
+        destruct U__r0; destruct U__r; simpl in *; subst;
+        churn;
+        [> do 3 eexists;
          repeat (apply conj);
          swap 3 4; swap 2 3; swap 1 2;
-           simpl; clean_map_lookups; simpl.
-
-        eapply Recd1; eauto.
-        unfold ideal_univ_start, ideal_univ_sent1, ideal_univ_recd1, ideal_univ_done, mkiU; simpl.
-        eapply TrcFront; simpl.
-        eapply IdealWorld.LStepUser'; simpl; swap 2 3; [ pick_user A | ..]; (try simple eapply @eq_refl).
-        unfold A , B; clean_map_lookups; eauto.
-        ((eapply IdealWorld.LStepBindRecur; i_single_silent_step) || i_single_silent_step); simpl.
-        solve_refl.
-
-        unfold ideal_univ_start, ideal_univ_sent1, ideal_univ_recd1, ideal_univ_done, mkiU; simpl; eauto 9.
-        
-      simpl_real_users_context.
-      simpl_ideal_users_context.
-      eapply Inp; simpl; auto.
-      eapply CryptoSigCase; simpl; eauto
-      econstructor.
-      intros.
-      split; intros; eauto.
-
-      apply lookup_some_implies_in in H0; simpl in H0; split_ors; try contradiction;
-        invert H0; clean_map_lookups; eauto.
-      simpl. unfold PERMS__a; clean_map_lookups; eauto.
-
-      apply lookup_some_implies_in in H0; simpl in H0; split_ors; try contradiction;
-        invert H0; clean_map_lookups; simpl; eauto.
-
-      unfold A , B in *; clean_map_lookups; simpl.
-      unfold A__keys; eauto.
-
-      + do 3 eexists;
-          repeat (apply conj);
-          swap 3 4; swap 2 3; swap 1 2;
-            simpl; clean_map_lookups;
-              eauto 9.
-        
-      simpl_real_users_context.
-      simpl_ideal_users_context.
-      eapply Inp; simpl; auto.
-      eapply CryptoSigCase; simpl; eauto.
-      econstructor.
-      intros.
-      split; intros; eauto.
-
-      apply lookup_some_implies_in in H1; simpl in H1; split_ors; try contradiction;
-        invert H1; clean_map_lookups; eauto.
-      simpl. unfold PERMS__a; clean_map_lookups; eauto.
-
-      apply lookup_some_implies_in in H2; simpl in H2; split_ors; try contradiction;
-        invert H2; clean_map_lookups; simpl; eauto.
-
-    - churn.
-
-    (* time *)
-    (*   (intros; *)
-    (*    invert H; *)
-    (*    try destruct U__r0; try destruct U__r; simpl in *; subst; *)
-    (*    churn; *)
-    (*    simpl_real_users_context; *)
-    (*    (* autorewrite with simpl_univ; *) *)
-    (*    (* simpl; *) *)
-    (*    (do 3 eexists; *)
-    (*     repeat (apply conj); *)
-    (*     swap 3 4; swap 2 3; swap 1 2; [ .. | admit (* action matches predicate *)]; *)
-    (*     simpl; clean_map_lookups; *)
-    (*     eauto; eauto 12)). *)
-
+         simpl; clean_map_lookups; eauto 12 ..]
+      ). repeat (solve_action_matches1; simpl; eauto).
   Qed.
-
-  Lemma rsimpleping_univere_ok :
-    simulates_universe_ok RSimplePing.
+  
+  Lemma rsimpleenc_honest_actions_safe :
+    honest_actions_safe Unit RSimpleEnc.
   Proof.
-    unfold simulates_universe_ok; intros.
+    unfold honest_actions_safe; intros. (* R UOK AOK LAME ** .*)
+    clear H1 H0.
+    inversion H; clear H;
+      destruct U__r0; destruct U__r; simpl in *; subst.
 
-    (* time ( *)
-    (*     inversion H; clear H; churn; solve_uok; eauto *)
-    (*   ). *)
+    - churn;
+        [> solve_honest_actions_safe; clean_map_lookups; eauto 8 .. ].
 
-  Admitted.
+    - churn;
+        [> solve_honest_actions_safe; clean_map_lookups; eauto 8 .. ].
 
-  Lemma rsimpleping_labeled_simulates_safe :
-    simulates_labeled_step_safe RSimplePing.
-  Proof.
-    unfold simulates_labeled_step_safe.
-    intros.
+    - churn;
+        [> solve_honest_actions_safe; clean_map_lookups; eauto 8 .. ].
 
-    (* assert (RealWorld.findUserKeys U__r.(RealWorld.users) = *)
-    (*         RealWorld.findUserKeys (clean_users (RealWorld.findUserKeys U__r.(RealWorld.users)) U__r.(RealWorld.users))) *)
-    (*   by (symmetry; eapply clean_users_no_change_findUserKeys). *)
-    (* remember (RealWorld.findUserKeys U__r.(RealWorld.users)) as honestk. *)
-
-    (* time( *)
-    (*     inversion H; clear H; *)
-    (*     churn; *)
-    (*     [> users_inversion; churn; repeat equality1; solve_adv_safe; eauto .. ] *)
-    (*   ). *)
-
-  Admitted.
-
-  (* Timings:
-   *
-   * --------------------------------------------------------------
-   * --------------------------------------------------------------
-   *)
-
+      Unshelve. all: eauto.
+  Qed.
+  
   Hint Resolve
-       rsimpleping_silent_simulates
-       rsimpleping_loud_simulates
-       rsimpleping_univere_ok
-       rsimpleping_labeled_simulates_safe.
+       rsimpleenc_silent_simulates
+       rsimpleenc_loud_simulates
+       rsimpleenc_honest_actions_safe : core.
 
   Lemma univ_ok_start :
     forall adv,
-      lameAdv tt adv
-      -> universe_ok (real_univ_start $0 [] [] [] [] [] [] 0 0 adv).
+      @lameAdv Unit tt adv
+      -> universe_ok (real_univ_start $0 [] [] 0 0 adv).
   Proof.
     unfold real_univ_start; econstructor; eauto.
   Qed.
 
+  Lemma merge_perms_true_either_true :
+    forall ks1 ks2 k_id,
+      ks1 $? k_id = Some true \/ ks2 $? k_id = Some true
+      -> ks1 $k++ ks2 $? k_id = Some true.
+  Proof.
+    intros; split_ors; solve_perm_merges.
+  Qed.
+
+  Hint Resolve merge_perms_true_either_true : core.
+
   Lemma adv_univ_ok_start :
     forall adv U__r honestk,
-      U__r = real_univ_start $0 [] [] [] [] [] [] 0 0 adv
+      U__r = real_univ_start $0 [] [] 0 0 adv
       -> honestk = RealWorld.findUserKeys U__r.(RealWorld.users)
-      -> lameAdv tt adv
-      -> adv.(RealWorld.msg_heap) = []
+      -> @lameAdv Unit tt adv
       -> adv.(RealWorld.key_heap) = $0
-      -> adv_universe_ok (real_univ_start $0 [] [] [] [] [] [] 0 0 adv).
+      -> adv.(RealWorld.msg_heap) = []
+      -> adv.(RealWorld.c_heap) = []
+      -> adv_universe_ok (real_univ_start $0 [] [] 0 0 adv).
   Proof.
     intros; unfold lameAdv in *;
-    unfold real_univ_start
-         , adv_universe_ok
-         , keys_and_permissions_good
-         , permission_heap_good.
-         
+      unfold real_univ_start, adv_universe_ok, keys_and_permissions_good, permission_heap_good.
     simpl; intuition (subst; eauto).
-
     - unfold KEYS in *; solve_simple_maps; eauto.
     - rewrite Forall_natmap_forall; intros;
         unfold A__keys, B__keys, KEYS in *;
         simpl in *; solve_simple_maps;
           simpl in *; solve_simple_maps;
             eauto.
-    - subst.
-
-
-    - unfold keys_good, KEYS, KID1, KID2, KEY1, KEY2; intros.
-      cases (0 ==n k_id); cases (1 ==n k_id); subst; clean_map_lookups; eauto.
-
+    - rewrite H2 in H5; clean_map_lookups.
+      
     - unfold user_cipher_queues_ok.
       rewrite Forall_natmap_forall; intros.
       cases (A ==n k); cases (B ==n k); subst; clean_map_lookups; simpl in *; econstructor; eauto.
@@ -442,23 +305,57 @@ Section FeebleSimulates.
       rewrite Forall_natmap_forall; intros.
       cases (A ==n k); cases (B ==n k); subst; clean_map_lookups; simpl in *; econstructor; eauto.
 
+    - unfold adv_cipher_queue_ok.
+      rewrite Forall_forall; intros.
+      rewrite H4 in H; contradiction.
+
+    - unfold adv_message_queue_ok.
+      rewrite Forall_forall; intros.
+      rewrite H3 in H; contradiction.
+
+    - unfold adv_no_honest_keys; intros.
+      rewrite !findUserKeys_add_reduce, findUserKeys_empty_is_empty; eauto.
+      unfold A__keys, B__keys; destruct (k_id ==n KID__A); destruct (k_id ==n KID__B); subst; solve_perm_merges.
+      + right. right. rewrite H2. split. eauto. clean_map_lookups.
+      + right; right. rewrite H2. split. eauto. clean_map_lookups.
+      + left. apply merge_perms_adds_no_new_perms; clean_map_lookups; eauto.
+
+    - unfold honest_nonces_ok; intros.
+      unfold honest_nonce_tracking_ok.
+
+      destruct (u_id ==n A); destruct (u_id ==n B);
+        destruct (rec_u_id ==n A); destruct (rec_u_id ==n B);
+          unfold A in *; unfold B in *;
+            subst; try contradiction; try discriminate;
+              clean_map_lookups; eauto; simpl; repeat (apply conj); intros;
+                clean_map_lookups; eauto.
+
+    - unfold honest_users_only_honest_keys; intros.
+      destruct (u_id ==n A); destruct (u_id ==n B);
+        subst; simpl in *; clean_map_lookups;
+          rewrite !findUserKeys_add_reduce, findUserKeys_empty_is_empty; eauto; simpl in *.
+      + unfold A__keys in H0; destruct (KID__A ==n k_id); destruct (KID__B ==n k_id);
+          subst; clean_map_lookups; eauto.
+      + unfold B__keys in H0; destruct (KID__A ==n k_id); destruct (KID__B ==n k_id);
+          subst; clean_map_lookups; eauto.
   Qed.
 
-  Hint Resolve
-       univ_ok_start
-       adv_univ_ok_start.
+  Hint Resolve univ_ok_start adv_univ_ok_start : core.
 
   Theorem base_pingpong_refines_ideal_pingpong :
     forall adv U__r honestk,
-      U__r = real_univ_start $0 [] [] adv
+      U__r = real_univ_start $0 [] [] 0 0 adv
       -> honestk = RealWorld.findUserKeys U__r.(RealWorld.users)
-      -> lameAdv tt adv
-      -> adv_message_queue_ok honestk adv.(RealWorld.msg_heap)
+      -> @lameAdv Unit tt adv
+      -> RealWorld.key_heap adv = $0
+      -> RealWorld.msg_heap adv = []
+      -> RealWorld.c_heap adv = []
+      -> adv_message_queue_ok U__r.(RealWorld.users) U__r.(RealWorld.all_ciphers) U__r.(RealWorld.all_keys) adv.(RealWorld.msg_heap)
       -> adv_no_honest_keys honestk adv.(RealWorld.key_heap)
       (* real_univ_start $0 [] [] adv <| ideal_univ_start / lameAdv tt. *)
-      -> refines (lameAdv tt) U__r ideal_univ_start.
+      -> refines (@lameAdv Unit tt) U__r ideal_univ_start.
   Proof.
-    exists RPingPongBase; unfold simulates.
+    exists RSimpleEnc; unfold simulates.
     intuition (subst; eauto).
   Qed.
 
